verif/verif_putrecord.v
@@ -66,14 +66,18 @@ Proof.
     destruct H. { exfalso. inv H. inv H7. }
     assert(HE: exists ke childe, e = keychild val ke childe).
     { simpl in H3. destruct e. simpl in H3. inv H3. exists k. exists n. auto. }
-    destruct HE as [ke [childe HE]]. 
+    destruct HE as [ke [childe HE]].
+    assert_PROP(isptr (getval childe)).
+    { rewrite HE. simpl entry_rep. entailer!. } rename H7 into ISPTRC.      
       
     forward_call(false,true,true). (* t'1=createnewnode(false,true,true) *)
     Intros vnewnode.
+    assert_PROP(isptr vnewnode).
+    entailer!. rename H7 into ISPTRV.
     gather_SEP 1 2. replace_SEP 0 (cursor_rep [] r pc).
     { entailer!. unfold cursor_rep. Exists anc_end. Exists idx_end. unfold r. cancel.
       change_compspecs CompSpecs. cancel. } clear anc_end. clear idx_end.
-    forward_if(PROP (vnewnode <> nullval) LOCAL (temp _currNode__1 vnewnode; temp _t'44 (Vint (Int.repr (-1))); temp _cursor pc; temp _newEntry pe; temp _key (key_repr oldk)) SEP (cursor_rep [] r pc; btnode_rep (empty_node false true true vnewnode); relation_rep (root, prel); entry_rep e; data_at Tsh tentry (entry_val_rep e) pe)).
+    forward_if(PROP (vnewnode <> nullval) LOCAL (temp _currNode__1 vnewnode; temp _t'44 (Vint (Int.repr (-1))); temp _cursor pc; temp _newEntry pe; temp _key (key_repr oldk)) SEP (cursor_rep [] r pc; btnode_rep (empty_node false true true vnewnode); relation_rep (root, prel) (get_numrec(root,prel) + entry_numrec e - 1); entry_rep e; data_at Tsh tentry (entry_val_rep e) pe)).
     + apply denote_tc_test_eq_split.
       replace (vnewnode) with (getval (empty_node false true true vnewnode)). entailer!.
       simpl. auto.
@@ -84,9 +88,29 @@ Proof.
     + unfold cursor_rep. Intros anc_end. Intros idx_end. unfold r.
       forward.                  (* t'52=cursor->relation *)
       unfold relation_rep. Intros.
+      assert_PROP(isptr (getval root)). { entailer!. } rename H8 into ISPTRR.
       forward.                  (* t'53=t'52->root *)
       unfold empty_node.
-      rewrite unfold_btnode_rep. Intros ent_end.
+      rewrite unfold_btnode_rep. Intros ent_end. simpl.
+      assert_PROP(Zlength ent_end = Z.of_nat Fanout).
+      { entailer!. simplify_value_fits in H14.
+        destruct H14, H20, H21, H22, H23.
+        (* Set Printing Implicit.  *) clear -H24.
+        assert(value_fits (tarray tentry 15) ent_end). auto.
+        simplify_value_fits in H. destruct H.
+        simpl in H. Check (reptype tentry). admit. }
+        (* assert(reptype tentry = val * (val + val)). *)
+        (* change_compspecs btrees.CompSpecs. auto. *)
+        (* simplify_value_fits in H24. destruct H24. *)
+        
+
+        (* apply value_fits_JMeq with (t:=(Tstruct _Entry noattr)) in H24. *)
+
+        (* (@reptype btrees.CompSpecs (Tstruct _Entry noattr)) *)
+        (* simplify_value_fits in H24. destruct H24. *)
+        (* apply value_fits_JMeq with (t:=) in H24. simplify_value_fits in H24. destruct H24.  *)
+        (* rewrite Fanout_eq. rewrite H24. simpl. auto. } *)
+      rename H8 into HENTEND.
       forward.                  (* currnode1->ptr0=t'53 *)
       forward.                  (* currnode1->numKeys=1 *)
       subst e. simpl.
@@ -114,29 +138,60 @@ Proof.
                              true
                              true
                              vnewnode).
-      forward_call(newroot,oldk,([]:cursor val),pc,(newroot,prel)). (* movetoKey(currnode_1,key,cursor,0 *)
+      forward_call(newroot,oldk,([]:cursor val),pc,(newroot,prel), (get_numrec (root,prel) + node_numrec childe - 1 + 1)%nat). (* movetoKey(currnode_1,key,cursor,0 *)
       unfold relation_rep. unfold newroot. simpl. fold newroot.
       * rewrite upd_Znth_same. rewrite upd_Znth_twice.
+        apply force_val_sem_cast_neutral_isptr in ISPTRV.
+        assert(force_val(sem_cast_pointer vnewnode) = vnewnode).
+        { inversion ISPTRV. rewrite H9. auto. }
+        assert(Vint (Int.add (Int.repr (Z.of_nat (get_numrec (root, prel) + node_numrec childe - 1))) (Int.repr 1)) = Vint (Int.repr (Z.of_nat (get_numrec (root, prel) + node_numrec childe - 1 + 1)))).        
+        { rewrite add_repr. apply f_equal. apply f_equal.
+          rewrite Nat2Z.inj_add. simpl. auto. }
+        assert(Vint (Int.add (Int.repr (Z.of_nat (get_depth (root, prel)))) (Int.repr 1)) = Vint (Int.repr (Z.pos (Pos.of_succ_nat (index.max_nat (node_depth childe) (node_depth root)))))).
+        { rewrite add_repr. repeat apply f_equal. rewrite Zpos_P_of_succ_nat.
+          unfold get_depth. simpl. simpl in H3. inversion H3. rewrite index.max_refl. omega. }
+        rewrite H8. rewrite H9. rewrite H10.
+        cancel.
+        unfold subcursor_rep.
+        Exists (upd_Znth 0 anc_end vnewnode).
+        Exists idx_end. Exists (-1).
+        simpl. cancel. rewrite unfold_btnode_rep with (n:=newroot). unfold newroot.
+        Exists (sublist 1 (Zlength ent_end) ent_end).
+        simpl.
+        assert(force_val(sem_cast_pointer(getval root)) = getval root).
+        { apply force_val_sem_cast_neutral_isptr in ISPTRR. inversion ISPTRR. rewrite H12. auto. }
+        assert(force_val(sem_cast_pointer(getval childe)) = getval childe).
+        { apply force_val_sem_cast_neutral_isptr in ISPTRC. inversion ISPTRC. rewrite H13. auto. }
+        rewrite H11. rewrite H12. rewrite upd_Znth0. cancel. change_compspecs CompSpecs. cancel.
+        rewrite HENTEND. rewrite Fanout_eq. simpl. omega.
+        rewrite HENTEND. rewrite Fanout_eq. simpl. omega.
       * split. auto. split. apply cons_integrity. auto. simpl in H4. auto.
         split. unfold correct_depth.
         assert(get_depth (newroot,prel)= node_depth newroot). unfold get_depth. simpl. auto. rewrite H8.
         assert(get_depth (root,prel) = node_depth root). unfold get_depth. simpl. auto.
         rewrite H9 in H0.
         simpl. simpl in H3. apply eq_add_S in H3. rewrite H3. rewrite index.max_refl. auto.
-        simpl. split. auto. apply cons_wf. auto. simpl in H2. auto.        
+        simpl. split. auto. apply cons_wf. auto. simpl in H2. auto.
       * forward.                (* return *)
-        admit.
-      
-
+        Exists ([vnewnode]:list val). entailer!.
+        destruct (putEntry val [] (root,prel) (keychild val ke childe) oldk [] nullval) as [newc newr] eqn:HNEW.
+        unfold relation_rep.
+        rewrite putEntry_equation. simpl. fold newroot.
+        assert((Vint (Int.repr (Z.of_nat (get_numrec (root, prel) + node_numrec childe - 1 + 1)))) = 
+               Vint (Int.repr (Z.of_nat (get_numrec (newroot, prel))))).
+        { repeat apply f_equal. unfold newroot. unfold get_numrec. simpl.
+          admit.                (* at least one record *)
+        } rewrite H14. cancel. 
   - forward.                    (* skip *)
     destruct c as [|[currnode entryidx] c'] eqn:HC.
-    { simpl in H0. exfalso. apply H3. rewrite Int.neg_repr. auto. }
-    forward_call(r,c,pc).       (* t'26=currnode(cursor) *)
+    { simpl in H0. exfalso. apply H6. rewrite Int.neg_repr. auto. }
+    forward_call(r,c,pc,(get_numrec (root, prel) + entry_numrec e - 1)%nat).       (* t'26=currnode(cursor) *)
     { unfold r. unfold cursor_rep. Exists anc_end. Exists idx_end. cancel. change_compspecs CompSpecs.
-      cancel. rewrite HC. simpl. cancel. }
+      cancel. rewrite HC. simpl. cancel. change_compspecs CompSpecs. cancel. }
     { rewrite HC. unfold r. split.
       destruct H. right. auto. left. unfold ne_partial_cursor.
-      destruct H. split; auto. split; auto. simpl. omega. auto. }
+      destruct H. split; auto. split; auto. simpl. omega.
+      unfold correct_depth. omega. }
     rewrite HC. simpl.
     assert(SUBNODE: subnode currnode root).
     { destruct H. destruct H. apply complete_cursor_subnode in H. simpl in H. auto.
@@ -203,46 +258,52 @@ Proof.
   forward_if(PROP (pc <> nullval)
      LOCAL (lvar _newEntry (Tstruct _Entry noattr) v_newEntry; temp _cursor pc;
      temp _key (key_repr key); temp _record (value_repr record))
-     SEP (data_at_ Tsh (Tstruct _Entry noattr) v_newEntry; relation_rep r; cursor_rep c r pc)).
+     SEP (data_at_ Tsh (Tstruct _Entry noattr) v_newEntry; relation_rep r (get_numrec r); cursor_rep c r pc)).
   - forward.                    (* skip *)
     entailer!.
   - assert_PROP(False). entailer!. contradiction.
   - fold tentry.
     forward.                    (* newentry.ptr.record=record *)
     forward.                    (* newentry.key=key *)
-    forward_call(c,pc,r,key).   (* gotokey(cursor,key) *)
+    forward_call(c,pc,r,key,get_numrec r).   (* gotokey(cursor,key) *)
+    admit.
     forward_call((goToKey c r key),pc,r,(keyval val key record (field_address tentry [UnionField _record; StructField _ptr] v_newEntry)), v_newEntry, key). (* putEntry(cursor,newEntry,key *)
     + unfold entry_rep, value_rep, value_repr.
       unfold_data_at 1%nat.
       erewrite field_at_Tunion with (t:=tentry) (gfs:=[StructField _ptr]) (v1:=(inr(Vint(Int.repr(v_ record))))) (p:=v_newEntry).
       2:reflexivity. 2:apply JMeq_refl.
       simpl. unfold withspacer. rewrite if_true by omega.
+      replace((get_numrec r + 1 - 1)%nat) with (get_numrec r) by omega. cancel.
       rewrite field_at_data_at with (gfs:=[UnionField _record; StructField _ptr]).
-      simpl. cancel.
+      simpl. cancel. unfold_data_at 1%nat. cancel.
+      simpl. admit.
     + split3; auto. left. apply gotokey_complete. auto.
+      split3; auto. simpl. unfold cursor_depth.
+      admit.
     + Intros newx.
       destruct(putEntry val (goToKey c r key) r) as [newc newr] eqn:HPUTENTRY.
-      forward_call(newc,pc,newr). (* RL_MoveToNext(cursor) *)
-      * cancel.
-      * apply gotokey_complete with (key:=key) in H.
-        split3.
-        eapply putentry_complete. eauto. eauto.
-        eapply putentry_depth. eauto. eauto. eauto.
-        split3.
-        eapply putentry_wf. eauto. auto. eauto.
-        eapply putentry_integrity. eauto. auto. eauto.
-        eapply putentry_numrec. eauto. auto. eauto.
-      * forward.                (* return *)
-        Exists newx.
-        Exists((field_address tentry [UnionField _record; StructField _ptr] v_newEntry)).
-        entailer!. unfold RL_PutRecord.
-        rewrite HPUTENTRY.
-        cancel. fold tentry. unfold value_rep.
-        eapply derives_trans.
-        2:eapply data_at_data_at_ with (v:=(key_repr key, inr (value_repr record))).
-        unfold_data_at 2%nat.
-        erewrite field_at_Tunion with (t:=tentry) (gfs:=[StructField _ptr]) (v1:=(inr(Vint(Int.repr(v_ record))))) (p:=v_newEntry).
-        2: reflexivity. 2: apply JMeq_refl.
-        simpl. unfold withspacer. rewrite if_true by omega. cancel.
-        rewrite field_at_data_at. simpl. cancel.
-Qed.
+Admitted.
+(*       forward_call(newc,pc,newr,get_numrec newr). (* RL_MoveToNext(cursor) *) *)
+(*       * cancel. *)
+(*       * apply gotokey_complete with (key:=key) in H. *)
+(*         split3. *)
+(*         eapply putentry_complete. eauto. eauto. *)
+(*         eapply putentry_depth. eauto. eauto. eauto. *)
+(*         split3. *)
+(*         eapply putentry_wf. eauto. auto. eauto. *)
+(*         eapply putentry_integrity. eauto. auto. eauto. *)
+(*         eapply putentry_numrec. eauto. auto. eauto. *)
+(*       * forward.                (* return *) *)
+(*         Exists newx. *)
+(*         Exists((field_address tentry [UnionField _record; StructField _ptr] v_newEntry)). *)
+(*         entailer!. unfold RL_PutRecord. *)
+(*         rewrite HPUTENTRY. *)
+(*         cancel. fold tentry. unfold value_rep. *)
+(*         eapply derives_trans. *)
+(*         2:eapply data_at_data_at_ with (v:=(key_repr key, inr (value_repr record))). *)
+(*         unfold_data_at 2%nat. *)
+(*         erewrite field_at_Tunion with (t:=tentry) (gfs:=[StructField _ptr]) (v1:=(inr(Vint(Int.repr(v_ record))))) (p:=v_newEntry). *)
+(*         2: reflexivity. 2: apply JMeq_refl. *)
+(*         simpl. unfold withspacer. rewrite if_true by omega. cancel. *)
+(*         rewrite field_at_data_at. simpl. cancel. *)
+(* Qed. *)
